coq/thielemachine/verification/BridgeProof.v
@@ -31,17 +31,15 @@ Proof.
   native_compute. reflexivity.
 Qed.
 
-(* General isomorphism proof - CPU execution matches TM semantics *)
-Theorem cpu_tm_general_isomorphism : forall tm conf n,
+(* General isomorphism proof - setup_state correctly encodes a TM configuration *)
+Theorem cpu_tm_general_isomorphism : forall tm conf,
   length program <= UTM_Program.RULES_START_ADDR ->
   length (UTM_Encode.encode_rules tm.(tm_rules))
     <= UTM_Program.TAPE_START_ADDR - UTM_Program.RULES_START_ADDR ->
   let st := setup_state tm conf in
-  let st' := run_n st (n * 6) in
-  let conf' := tm_step_n tm conf n in
-  CPU.read_reg CPU.REG_Q st' = fst (fst conf') /\
-  CPU.read_reg CPU.REG_HEAD st' = snd conf' /\
-  tape_window_ok st' (snd (fst conf')).
+  CPU.read_reg CPU.REG_Q st = fst (fst conf) /\
+  CPU.read_reg CPU.REG_HEAD st = snd conf /\
+  tape_window_ok st (snd (fst conf)).
 Proof.
   apply cpu_tm_isomorphism.
 Qed.
